

## Mathematical analysis II

### Homework 3

To be handed in by Wednesday, 29.10.25, 23:59 h via OWL

---

#### Exercise 1 (Chain rule and extrema).

(2+2+2=6 points)

a) Let  $f : \mathbb{R} \rightarrow \mathbb{R}$  be differentiable. Show that for  $z = f(\frac{xy}{x^2+y^2})$  it holds

$$x\partial_x z + y\partial_y z = 0.$$

b) Let  $f : \mathbb{R} \rightarrow \mathbb{R}$  be differentiable and  $a \in \mathbb{R}^n$  and  $b \in \mathbb{R}$  be constant. Calculate the gradient of the function  $g : \mathbb{R}^n \rightarrow \mathbb{R}$ ,  $g(x) = f(\langle a, x \rangle + b)$ . Here, the notation  $\langle a, x \rangle$  is the scalar product of these vectors. Remember that the gradient is defined as  $\nabla g = (\partial_{x_1} g, \dots, \partial_{x_n} g)$ .

c) Let

$$f(x, y) = (x - y - 1)^2.$$

Find and classify all extrema (minimum/maximum/saddle point).

**Solution.** a) We have

$$\begin{aligned}\partial_x z &= f' \left( \frac{xy}{x^2+y^2} \right) \frac{y(x^2+y^2) - 2x^2y}{(x^2+y^2)^2}, \\ \partial_y z &= f' \left( \frac{xy}{x^2+y^2} \right) \frac{x(x^2+y^2) - 2y^2x}{(x^2+y^2)^2}.\end{aligned}$$

In turn,

$$\begin{aligned}x\partial_x z + y\partial_y z &= f' \left( \frac{xy}{x^2+y^2} \right) \left[ x \frac{y(x^2+y^2) - 2x^2y}{(x^2+y^2)^2} + y \frac{x(x^2+y^2) - 2y^2x}{(x^2+y^2)^2} \right] \\ &= f' \left( \frac{xy}{x^2+y^2} \right) \frac{x^3y + xy^3 - 2x^3y + x^3y + xy^3 - 2xy^3}{(x^2+y^2)^2} = 0.\end{aligned}$$

There is another nice proof that avoids fractions: define  $u(x, y) = \frac{xy}{x^2+y^2}$ . Then for any  $k \neq 0$  we have  $u(kx, ky) = u(x, y)$ . Now fix  $(x, y)$  and define for these (now fixed) points the function  $g(k) = u(kx, ky)$ . But then  $g(k) = u(kx, ky) = u(x, y)$ , so  $g$  is a constant function of  $k$  (since  $(x, y)$  is fixed). This means  $g'(k) = 0$ , where the derivative is wrt.  $k$ . Now let's apply chain rule:

$$0 = g'(k) = x\partial_x u(kx, ky) + y\partial_y u(kx, ky).$$

Taking the above equality in  $k = 1$  and noting also that, again by chain rule, we have  $x\partial_x z + y\partial_y z = f'(u)(x\partial_x u + y\partial_y u)$ , this shows the desired.

b) According to chain rule, we get

$$\nabla g(x) = f'(\langle a, x \rangle + b) \nabla(\langle a, x \rangle + b) = f'(\langle a, x \rangle + b) \nabla \langle a, x \rangle$$

since  $b$  is constant and hence  $\nabla b = 0$ . Further for any  $i \in \{1, \dots, n\}$

$$\partial_{x_i} \langle a, x \rangle = \partial_{x_i} \sum_{j=1}^n a_j x_j = a_i$$

such that simply  $\nabla \langle a, x \rangle = a$  and thus

$$\nabla g(x) = f'(\langle a, x \rangle + b) a.$$

Note that since  $a$  is a vector, also the right hand-side is. Compare this with the one-dimensional rule  $[f(ax + b)]' = af'(ax + b)$ . (Note: to be fully correct we would need to write  $\nabla g(x) = f'(\langle a, x \rangle + b) a^T$  since  $\nabla g$  is a row vector; but as I said in class, there is not really a common style how to write it.)

c) We calculate

$$\nabla f(x, y) = (2(x - y - 1), -2(x - y - 1))$$

and thus  $\nabla f = 0$  iff  $y = x - 1$ . Since  $f$  is quadratic, in particular  $f(x, y) \geq 0$  for any pair  $(x, y) \in \mathbb{R}^2$ , and  $f(x, x - 1) = 0$ , all points of the form  $(x, x - 1)$  are (global) minima. (And, since points  $(x, x - 1)$  are the only critical points who are all minima, no maxima or saddle points exist.)

## Exercise 2 (Derivatives of higher order).

(2+2=4 points)

a) Calculate for the following function the derivatives up to second order:

$$f(x, y) = (x + y + 3)^2 - e^{2x+y^2}.$$

b) For the vectorial function  $v = (v_1, v_2, v_3) : \mathbb{R}^3 \rightarrow \mathbb{R}^3$  we define the divergence and curl via

$$\operatorname{div} v = \nabla \cdot v = \partial_1 v_1 + \partial_2 v_2 + \partial_3 v_3,$$

$$\operatorname{curl} v = \nabla \times v = \begin{pmatrix} \partial_2 v_3 - \partial_3 v_2 \\ \partial_3 v_1 - \partial_1 v_3 \\ \partial_1 v_2 - \partial_2 v_1 \end{pmatrix}.$$

(Here  $\partial_i v_j$  means  $\partial v_j / \partial x_i$  for any  $i, j \in \{1, 2, 3\}$ .) Show that  $\operatorname{div} \operatorname{curl} v = 0$ .

**Solution.** a) We have

$$\begin{aligned} \partial_x f &= 2(x + y + 3) - 2e^{2x+y^2}, & \partial_y f &= 2(x + y + 3) - 2ye^{2x+y^2}, \\ \partial_{xy}^2 f &= 2 - 4ye^{2x+y^2} = \partial_{yx}^2 f, \\ \partial_{xx}^2 f &= 2 - 4e^{2x+y^2}, & \partial_{yy}^2 f &= 2 - 2e^{2x+y^2} - 4y^2 e^{2x+y^2}. \end{aligned}$$

Here, we also have  $\partial_{xy}^2 f = \partial_{yx}^2 f$  by Schwarz' theorem (note that the second mixed partial derivatives are continuous).

b) Calculation and re-arranging leads to

$$\begin{aligned}\operatorname{div} \operatorname{curl} v &= \partial_1(\partial_2 v_3 - \partial_3 v_2) + \partial_2(\partial_3 v_1 - \partial_1 v_3) + \partial_3(\partial_1 v_2 - \partial_2 v_1) \\ &= \partial_{12}^2 v_3 - \partial_{21}^2 v_3 + \partial_{23}^2 v_1 - \partial_{32}^2 v_1 + \partial_{31}^2 v_2 - \partial_{13}^2 v_2 = 0.\end{aligned}$$

Especially here, we used Schwarz' theorem to see that  $\partial_{ij}^2 v_k = \partial_{ji}^2 v_k$ . In a similar way one can show that  $\operatorname{curl} \nabla f = 0$  for any (differentiable)  $f : \mathbb{R}^3 \rightarrow \mathbb{R}$ . Such things are very often used in physics, mainly when talking about magnetic fields, and in some special cases, also the other direction holds: if  $v : U \rightarrow \mathbb{R}^3$  is a function, where  $U \subset \mathbb{R}^3$  is "not too bad", and if  $\operatorname{div} v = 0$ , then there exists some vector-valued function  $w : U \rightarrow \mathbb{R}^3$  such that  $v = \operatorname{curl} w$ . For instance the magnetic field  $B$  is always source-free (there are no magnetic monopoles), which means exactly  $\operatorname{div} B = 0$ , and there exists some so-called vector potential  $A$  such that  $B = \operatorname{curl} A$ . From this the whole theory about magnetic fields follows, how stars are working, etc.